Tests/Grammar/Core.lean
@@ -12,4 +12,22 @@ example (byte : Byte) (suffix : Std.Logical.ByteArray) :
     Derives (.byte (fun _ => True)) (Vec.singleton byte ++ suffix) byte suffix :=
   Derives.byte (fun _ => True) byte suffix trivial
 
+def exactlyTwoBytes : Format (Vec Byte) :=
+  .repeat 2 (.byte (fun _ => True))
+
+example (first second : Byte) (suffix : Std.Logical.ByteArray) :
+    Derives exactlyTwoBytes
+      (Vec.singleton first ++ Vec.singleton second ++ suffix)
+      (Vec.fromList [first, second]) suffix := by
+  apply Derives.repeatSucc
+  · exact Derives.byte (fun _ => True) first _ trivial
+  · apply Derives.repeatSucc
+    · exact Derives.byte (fun _ => True) second suffix trivial
+    · exact Derives.repeatZero (.byte (fun _ => True)) suffix
+
+example (byte : Byte) (suffix : Std.Logical.ByteArray) :
+    Derives (.iso (.byte (fun _ => True)) (Isomorphism.refl Byte))
+      (Vec.singleton byte ++ suffix) byte suffix :=
+  Derives.iso (Derives.byte (fun _ => True) byte suffix trivial)
+
 end Grass.Tests.Grammar
